WIP

proof/spec/extra/SpecSecurity.ec
@@ -72,11 +72,14 @@ op pkrel(apk : pkXMSSTW, pk : xmss_pk) =
   we exit the loop, where everything works in a tree of height h+1
 *)
 
+type path = bool list.
+
 (* The hamming weight of a path determines the size of the stack *)
-op hw(p : bool list) = count (pred1 true) p.
+op hw (p : path) = count (pred1 true) p.
 
 (* The path of a leaf; we need the corner case of leaf 2^h for exiting the loop *)
-op lpath(lidx : int) = rev (BS2Int.int2bs (if lidx = 2^h then (h+1) else h) lidx).
+op lpath (lidx : int) =
+  rev (BS2Int.int2bs (h + (b2i (lidx = 2^h))) lidx).
 
 (*
                      +
@@ -90,39 +93,38 @@ path to 6 = 1 1 0 => stack contains [0] and [1 0]
 *)
 
 (* The paths of all the sibling nodes of 1-bit choices in a leaf path *)
-op paths_from_leaf(lidx : int) : bool list list =
-   if (lidx = 2^h) then [[]] (* we get the root *)
-   else pmap (fun (bi : _*_) =>
-     if bi.`1
-     then Some ((take bi.`2 (lpath lidx)) ++ [false])
-     else None) (zip (lpath lidx) (iota_ 0 h)).
+op paths_from_leaf (lidx : int) : path list =
+  if (lidx = 2^h) then [[]] (* we get the root *) else
+
+  pmap (fun i =>
+    let p = take i (lpath lidx) in
+    if   last false p
+    then Some (take (i - 1) p ++ [false])
+    else None
+  ) (range 0 h).
 
 lemma size_lpath (lidx) :
    lidx <= 2^h =>
      size (lpath lidx) = if lidx = 2^h then (h+1) else h.
-move => H.
-rewrite /lpathl size_rev BS2Int.size_int2bs; smt(h_g0).
+proof.
+by move=> hle @/lpath; rewrite size_rev BS2Int.size_int2bs; smt(h_g0).
 qed.
 
 (* Move to List *)
-lemma count_eq_nth ['a] (p : 'a -> bool) :
-   forall (s : int) (s1 s2 : 'a list), 
-   size s1 = s =>   size s2 = s =>
-   (forall k, 0 <= k < s =>
-      p (nth witness s1 k) = p (nth witness s2 k)) =>
-        count p s1 = count p s2.
+lemma count_eq_nth ['a] (p : 'a -> bool) (s1 s2 : 'a list) :
+     size s1 = size s2
+  => (forall k, 0 <= k < size s1 => p (nth witness s1 k) = p (nth witness s2 k))
+  => count p s1 = count p s2.
 proof. 
-move => s.
-elim /natind:s; 1: by smt(size_ge0 count_size).
-move => n nge0 Hi s1 s2 Hs1 Hs2 Hp.
-rewrite -(head_behead  s1 witness) 1:/# -(head_behead  s2 witness) 1:/# /=.
-congr; 1: by smt(mem_head).
-by apply (Hi (behead s1) (behead s2));smt(size_behead nth_behead).
+elim: s1 s2 => [|x1 s1 ih] [|x2 s2] //=; ~-1:smt(size_ge0).
+by move/addzI => eq_sz heqp; rewrite (heqp 0) ?(ih s2); smt(size_ge0).
 qed.
 
 lemma pfl_size (lidx : int) :
    lidx <= 2^h =>
    size (paths_from_leaf lidx) = hw (lpath lidx).
+proof.
+(*
 rewrite /paths_from_leaf => Hs.
 case (lidx = 2 ^ h) => /= Hh.
 + rewrite /lpath /= Hh /= /hw BS2Int.int2bs_pow2;1:smt(mem_range h_g0).
@@ -138,7 +140,8 @@ have -> : count (pred1 true) (lpath lidx) =
     count (pred1 true) (unzip1  (zip (lpath lidx) (iota_ 0 (size (lpath lidx))))).
 + by congr;rewrite unzip1_zip;1:smt(size_iota size_ge0). 
 by rewrite count_map;apply eq_in_count => x memx /= /#.
-qed.
+*)
+admitted.
 
 (* The list of leaves that are under a node given by a path *)
 op leaves_from_path(p : bool list) =
@@ -157,7 +160,7 @@ rewrite /leaves_from_path ifF /=;1:
       smt(StdOrder.IntOrder.expr_ge0 h_g0).
 rewrite size_lpath 1:/# /= ifF 1:/# /= iota1;congr.
 admit. (* annoying *)
-qed.
+admitted.
 
 (* The leaf node corresponding to a leaf path
    The semantics of this needs to be computed from wots using
@@ -166,7 +169,7 @@ op leafnode_from_idx(ss ps : Params.nbytes, ad : SA.adrs, lidx : int) : dgstbloc
 
 (* list of all the leaves up to an index, exclusive *)
 op leaf_range(ss ps : Params.nbytes, ad : SA.adrs, lidx : int) =
-   map (leafnode_from_idx ss ps ad) (iota_ 0 lidx).
+   map (leafnode_from_idx ss ps ad) (range 0 lidx).
 
 (* The node corresponding to an arbitrary path  *)
 op node_from_path(p : bool list,ss ps : Params.nbytes, ad : SA.adrs) : dgstblock =
@@ -187,6 +190,7 @@ lemma sfl_size lidx ss ps ad :
   lidx <= 2^h =>
   size (stack_from_leaf lidx ss ps ad) = hw (lpath lidx).
 proof.
+(*
 move => Hi.
 rewrite  /stack_from_leaf size_map /paths_from_leaf.
 case (lidx = 2 ^ h) => H /=.
@@ -203,7 +207,8 @@ have -> : count (pred1 true) (lpath lidx) =
     count (pred1 true) (unzip1  (zip (lpath lidx) (iota_ 0 (size (lpath lidx))))).
 + by congr;rewrite unzip1_zip;1:smt(size_iota size_ge0). 
 by rewrite count_map;apply eq_in_count => x memx /= /#.
-qed.
+*)
+admitted.
 
 (* The list of leaves that fall under the first node in the stack when one starts to process leaf lidx
    The case o lidx=0 is a corner case, as the stack is empty *)
@@ -216,12 +221,15 @@ op first_subtree_leaves(lidx : int,ss ps : Params.nbytes, ad : SA.adrs) =
 
 (* The hamming weight of 0 is 0, so stack is empty *)
 lemma pfl0 : paths_from_leaf 0 = [].
+proof.
+(*
 rewrite /paths_from_leaf ifF;1:smt(StdOrder.IntOrder.expr_gt0 h_g0).
 rewrite (eq_in_pmap _ (fun _ => None)).
 + move => bi H; have := mem_zip  (lpath 0) (iota_ 0 h) bi.`1 bi.`2 _; 1:smt().
   rewrite /lpath mem_rev BS2Int.int2bs0 mem_nseq /#.
 by apply pmap_none.
-qed.
+*)
+admitted.
 
 (* This op describes the state of the stack in the inner loop, while
    reducing, where i is the number of the iteration we are in.
